---
title: "formulas"
author: "Shinichi Nakagawa"
date: "17/05/2021"
output:
  word_document: default
  html_document: default
---


$$
\ln{\text{RR}} = \ln \left( \frac{m_{T}} {m_{C}}\right) + 
\frac{1}{2} \left(\frac{\text{CV}_T^2} {n_{T}} - \frac{\text{CV}_C^2} {n_{C}}\right), 
$$


$$
v(\ln{\text{RR}}) = \frac{\text{CV}_T^2} {n_{T}} + \frac{\text{CV}_C^2} {n_{C}} - 2r_{TC}\frac{\text{CV}_T \text{CV}_C}{\sqrt{n_Cn_T}},
$$
$n_{T} = n_{C} = n$

$\text{CV}_C = sd_T/m_T$ and $\text{CV}_C = sd_C/m_C$


$$
\ln{\text{RR}} = \ln \left( \frac{m_{T}} {m_{C}}\right) + 
\frac{1}{2} \left(\frac{\sum_{i=1}^{k}{\text{CV}_{Ti}^2}/k} {n_{T}} - \frac{\sum_{i=1}^{k}{\text{CV}_{Ci}^2}/k} {n_{C}}\right), 
$$


$$
v(\ln{\text{RR}})= \frac{\sum_{i=1}^{k}{\text{CV}_{Ti}^2}/k} {n_{T
}} + \frac{\sum_{i=1}^{k}{\text{CV}_{Ci}^2}/k} {n_{C}} - 2r_{TC}\frac{(\sum_{i=1}^{k}{\text{CV}_{Ti}^2}/k) (\sum_{i=1}^{k}{\text{CV}_{Ci}^2}/k)}{\sqrt{n_T n_C}},
$$




